added constant, renamed erased to roleing

src/FcEtt/ett_par.v
@@ -13,7 +13,7 @@ Require Export FcEtt.ett_ind.
 Require Export FcEtt.ext_context_fv.
 
 Require Import FcEtt.ext_wf.
-Require Import FcEtt.ett_erased.
+Require Import FcEtt.ett_roleing.
 Require Import FcEtt.ett_path.
 Import ext_wf.
 Require Import FcEtt.param.
@@ -31,7 +31,7 @@ Lemma par_app_rctx : forall W1 W2 W3 a a' R, uniq (W1 ++ W2 ++ W3) ->
                      Par (W1 ++ W2 ++ W3) a a' R.
 Proof. intros W1 W2 W3 a a' R U H. generalize dependent W2.
        dependent induction H; intros; eauto.
-       all: try solve [econstructor; eauto 3 using erased_app_rctx].
+       all: try solve [econstructor; eauto 3 using roleing_app_rctx].
         - eapply Par_Abs with (L := union L (dom (W1 ++ W2 ++ W3))).
           intros. rewrite <- app_assoc.
           eapply H0; eauto. simpl_env. auto.
@@ -50,7 +50,7 @@ Qed.
 (* TODO: move these definitions to the OTT file. *)
 
 Inductive multipar W ( a : tm) : tm -> role -> Prop :=
-| mp_refl : forall R, erased_tm W a R -> multipar W a a R
+| mp_refl : forall R, roleing W a R -> multipar W a a R
 | mp_step : forall R b c, Par W a b R -> multipar W b c R -> 
                                              multipar W a c R.
 
@@ -61,14 +61,14 @@ Lemma multipar_app_rctx : forall W1 W2 W3 a a' R, uniq (W1 ++ W2 ++ W3) ->
                      multipar (W1 ++ W2 ++ W3) a a' R.
 Proof. intros W1 W2 W3 a a' R U H. generalize dependent W2.
        dependent induction H; intros; eauto.
-        - econstructor. eapply erased_app_rctx; eauto.
+        - econstructor. eapply roleing_app_rctx; eauto.
         - econstructor; eauto. apply par_app_rctx; auto.
 Qed.
 
 Definition joins W a b R := exists c, multipar W a c R /\ multipar W b c R.
 
 Lemma Par_lc1 : forall W a a' R , Par W a a' R -> lc_tm a.
-  intros.  induction H; auto; eapply erased_lc; eauto.
+  intros.  induction H; auto; eapply roleing_lc; eauto.
 Qed.
 
 (* FIXME: find a good place for this tactic. *)
@@ -94,52 +94,53 @@ Qed.
 
 Hint Resolve Par_lc1 Par_lc2 : lc.
 
-Lemma Par_erased_tm_fst : forall W a a' R, Par W a a' R -> 
-                                               erased_tm W a R.
+Lemma Par_roleing_tm_fst : forall W a a' R, Par W a a' R -> 
+                                               roleing W a R.
 Proof. intros W a a' R H. induction H; eauto.
-       apply Path_binds_toplevel in H2. inversion H2 as [a0 [A0 [R1 P]]].
-       econstructor; eauto.
+       apply Path_binds_toplevel in H2.
+       inversion H2 as [[A P] | [a0 [A0 [R1 P]]]]. eauto.
+       inversion P. eauto.
 Qed.
 
-Lemma multipar_erased_tm_fst: forall W a a' R, multipar W a a' R -> 
-                                               erased_tm W a R.
-Proof. intros. induction H. auto. eapply Par_erased_tm_fst; eauto.
+Lemma multipar_roleing_tm_fst: forall W a a' R, multipar W a a' R -> 
+                                               roleing W a R.
+Proof. intros. induction H. auto. eapply Par_roleing_tm_fst; eauto.
 Qed.
 
-Lemma Par_erased_tm_snd : forall W a a' R, Par W a a' R ->
-                                               erased_tm W a' R.
+Lemma Par_roleing_tm_snd : forall W a a' R, Par W a a' R ->
+                                               roleing W a' R.
 Proof. intros W a a' R H. induction H; eauto.
         - inversion IHPar1; subst. pick fresh x.
           erewrite tm_subst_tm_tm_intro; eauto.
-          replace W with (nil ++ W); auto. eapply subst_tm_erased; eauto.
-          eapply erased_sub with (R1 := (param R1 R)); auto.
+          replace W with (nil ++ W); auto. eapply subst_tm_roleing; eauto.
+          eapply roleing_sub with (R1 := (param R1 R)); auto.
           apply param_sub1; auto.
         - inversion IHPar; subst. pick fresh c.
           erewrite co_subst_co_tm_intro; eauto.
-          replace W with (nil ++ W); auto. eapply subst_co_erased; eauto.
-        - eapply erased_sub. eapply toplevel_erased1; eauto. auto.
+          replace W with (nil ++ W); auto. eapply subst_co_roleing; eauto.
+        - eapply roleing_sub. eapply toplevel_roleing1; eauto. auto.
 Qed.
 
-Lemma multipar_erased_tm_snd : forall W a a' R, multipar W a a' R ->
-                                               erased_tm W a' R.
+Lemma multipar_roleing_tm_snd : forall W a a' R, multipar W a a' R ->
+                                               roleing W a' R.
 Proof. intros. induction H; auto.
 Qed.
 
 Lemma Par_rctx_uniq : forall W a a' R, Par W a a' R -> uniq W.
-Proof. intros. eapply rctx_uniq. eapply Par_erased_tm_fst; eauto.
+Proof. intros. eapply rctx_uniq. eapply Par_roleing_tm_fst; eauto.
 Qed.
 
 Lemma multipar_rctx_uniq: forall W a a' R, multipar W a a' R -> uniq W.
-Proof. intros. eapply rctx_uniq. eapply multipar_erased_tm_fst; eauto.
+Proof. intros. eapply rctx_uniq. eapply multipar_roleing_tm_fst; eauto.
 Qed.
 
 Lemma par_multipar: forall W a a' R, Par W a a' R -> 
                                          multipar W a a' R.
 Proof. intros. eapply mp_step. eauto. constructor. 
-       eapply Par_erased_tm_snd; eauto.
+       eapply Par_roleing_tm_snd; eauto.
 Qed. 
 
-Hint Resolve Par_erased_tm_fst Par_erased_tm_snd : erased.
+Hint Resolve Par_roleing_tm_fst Par_roleing_tm_snd : roleing.
 
 (* ------------------------------------------------------------- *)
 
@@ -147,21 +148,21 @@ Lemma Par_sub: forall W a a' R1 R2, Par W a a' R1 -> SubRole R1 R2 ->
                                       Par W a a' R2.
 Proof. intros W a a' R1 R2 H SR. generalize dependent R2.
        induction H; intros; simpl; eauto using param_covariant. econstructor.
-       eapply erased_sub; eauto.
+       eapply roleing_sub; eauto.
 Qed.
 
 Lemma multipar_sub : forall W a a' R1 R2, multipar W a a' R1 ->
                      SubRole R1 R2 -> multipar W a a' R2.
-Proof. intros. induction H. econstructor. eapply erased_sub; eauto.
+Proof. intros. induction H. econstructor. eapply roleing_sub; eauto.
        econstructor; eauto. eapply Par_sub; eauto.
 Qed.
 
 Lemma subst1 : forall b W W' a a' R1 R2 x, Par W' a a' R1 -> 
-               erased_tm (W ++ [(x,R1)] ++ W') b R2 ->
+               roleing (W ++ [(x,R1)] ++ W') b R2 ->
                Par (W ++ W') (tm_subst_tm_tm a x b) (tm_subst_tm_tm a' x b) R2.
 Proof.
-  intros b W W' a a' R1 R2 x PAR ET.
-  dependent induction ET; intros; simpl; auto.
+  intros b W W' a a' R1 R2 x PAR RJ.
+  dependent induction RJ; intros; simpl; auto.
    - constructor. constructor. eapply uniq_remove_mid; eauto.
    - constructor. constructor. eapply uniq_remove_mid; eauto.
    - destruct (x0 == x); auto.
@@ -198,10 +199,11 @@ Proof.
    - econstructor; eauto.
    - econstructor; eauto.
    - econstructor; eauto.
+   - econstructor; eauto.
 Qed.
 
 Lemma open1 : forall b W L a a' R, Par W a a' R
-  -> (forall x, x `notin` L -> erased_tm W (open_tm_wrt_tm b (a_Var_f x)) R)
+  -> (forall x, x `notin` L -> roleing W (open_tm_wrt_tm b (a_Var_f x)) R)
   -> Par W (open_tm_wrt_tm b a) (open_tm_wrt_tm b a') R.
 Proof.
   intros.
@@ -209,46 +211,46 @@ Proof.
   rewrite (tm_subst_tm_tm_intro x); auto.
   rewrite [(_ _ a')] (tm_subst_tm_tm_intro x); auto.
   replace W with (nil ++ W); auto. eapply subst1; eauto.
-  apply erased_app_rctx; simpl_env.
+  apply roleing_app_rctx; simpl_env.
   constructor; auto. eapply Par_rctx_uniq; eauto.
   auto.
 Qed.
 
 Lemma subst2 : forall b W W' a a' R R1 x, 
           Par (W ++ [(x,R1)] ++ W') a a' R -> 
-          erased_tm W' b R1 ->
+          roleing W' b R1 ->
           Par (W ++ W') (tm_subst_tm_tm b x a) (tm_subst_tm_tm b x a') R.
 Proof.
   intros b W W' a a' R R1 x PAR E.
   dependent induction PAR; simpl. 
   all: eauto using tm_subst_tm_tm_lc_tm.
   all: autorewrite with subst_open; eauto.
-  all: try eapply erased_lc; eauto.
-  - econstructor. eapply subst_tm_erased; eauto.
+  all: try eapply roleing_lc; eauto.
+  - econstructor. eapply subst_tm_roleing; eauto.
   - eapply Par_Abs with (L := union L (singleton x)).
     intros x0 H1.
     rewrite tm_subst_tm_tm_open_tm_wrt_tm_var; auto 1.
     rewrite tm_subst_tm_tm_open_tm_wrt_tm_var; auto 1.
     rewrite <- app_assoc. eapply H0. auto. simpl_env; auto.
-    auto. eapply erased_lc; eauto. eapply erased_lc; eauto.
+    auto. eapply roleing_lc; eauto. eapply roleing_lc; eauto.
   - eapply Par_Pi with (L := union L (singleton x)); eauto.
     intros x0 H2.
     rewrite tm_subst_tm_tm_open_tm_wrt_tm_var; auto 1.
     rewrite tm_subst_tm_tm_open_tm_wrt_tm_var; auto 1.
     rewrite <- app_assoc. eapply H0. auto. simpl_env; auto.
-    auto. eapply erased_lc; eauto. eapply erased_lc; eauto.
+    auto. eapply roleing_lc; eauto. eapply roleing_lc; eauto.
   - eapply Par_CAbs with (L := union L (singleton x)).
     intros x0 H1.
     rewrite tm_subst_tm_tm_open_tm_wrt_co_var; auto 1.
     rewrite tm_subst_tm_tm_open_tm_wrt_co_var; auto 1.
     eapply H0. auto. eauto. auto.
-    eapply erased_lc; eauto. eapply erased_lc; eauto.
+    eapply roleing_lc; eauto. eapply roleing_lc; eauto.
   - eapply Par_CPi with (L := union L (singleton x)); eauto.
     intros x0 H4.
     rewrite tm_subst_tm_tm_open_tm_wrt_co_var; auto 1.
     rewrite tm_subst_tm_tm_open_tm_wrt_co_var; auto 1.
     eapply H0. auto. eauto. auto.
-    eapply erased_lc; eauto. eapply erased_lc; eauto.
+    eapply roleing_lc; eauto. eapply roleing_lc; eauto.
   - eapply Par_Axiom; eauto. 
     rewrite tm_subst_tm_tm_fresh_eq. eauto.
     apply toplevel_closed in H.
@@ -256,10 +258,10 @@ Proof.
     split_hyp. simpl in *.
     fsetdec.
   - eapply Par_PatternTrue; eauto. eapply Path_subst; eauto.
-    eapply erased_lc; eauto.
+    eapply roleing_lc; eauto.
   - eapply Par_PatternFalse; eauto.
-    eapply Value_tm_subst_tm_tm; eauto. eapply erased_lc; eauto.
-    intro. eapply subst_Path in H2; eauto. eapply erased_lc; eauto.
+    eapply Value_tm_subst_tm_tm; eauto. eapply roleing_lc; eauto.
+    intro. eapply subst_Path in H2; eauto. eapply roleing_lc; eauto.
 Qed.
 
 
@@ -269,7 +271,7 @@ Lemma subst3 : forall b b' W W' a a' R R1 x,
           Par (W ++ W') (tm_subst_tm_tm b x a) (tm_subst_tm_tm b' x a') R.
 Proof.
   intros.
-  dependent induction H; simpl; eauto 2; erased_inversion; eauto 4.
+  dependent induction H; simpl; eauto 2; roleing_inversion; eauto 4.
   all: try solve [ Par_pick_fresh y;
               autorewrite with subst_open_var; eauto 3 with lc ].
   all: try solve [ autorewrite with subst_open; eauto 4 with lc ].
@@ -309,7 +311,7 @@ Proof.
   all: try solve [ Par_pick_fresh y;
               autorewrite with subst_open_var; eauto 3 with lc ].
   all: try solve [ autorewrite with subst_open; eauto 4 with lc ].
-  - apply Par_Refl. eapply subst_co_erased; eauto.
+  - apply Par_Refl. eapply subst_co_roleing; eauto.
   - rewrite co_subst_co_tm_fresh_eq. eauto.
     apply toplevel_closed in H.
     apply Typing_context_fv in H.
@@ -328,14 +330,14 @@ Proof.
   intros b b' W W' a a' R R1 x H1 H2.
   dependent induction H1; auto.
   - dependent induction H2; auto.
-    constructor. eapply subst_tm_erased; eauto.
+    constructor. eapply subst_tm_roleing; eauto.
     apply (@mp_step _ _ _ ((tm_subst_tm_tm b x a))); auto.
     eapply subst3; eauto.
   - dependent induction H2; auto.
     apply (@mp_step _ _ _ (tm_subst_tm_tm a0 x b0)); auto.
     eapply subst3; eauto.
     apply (@mp_step _ _ _ ((tm_subst_tm_tm a0 x b0))); auto.
-    eapply subst2; eauto. eapply Par_erased_tm_fst; eauto.
+    eapply subst2; eauto. eapply Par_roleing_tm_fst; eauto.
     apply IHmultipar; auto.
     econstructor; eauto.
 Qed.
@@ -346,19 +348,19 @@ Lemma multipar_subst4 : forall W b x, lc_co b ->
 Proof.
   intros W b x H a a' R H0.
   dependent induction H0; eauto.
-  constructor. eapply subst_co_erased; eauto.
+  constructor. eapply subst_co_roleing; eauto.
   apply (@mp_step _ _ _ (co_subst_co_tm b x b0)); auto.
   apply subst4; auto.
 Qed.
 
-Lemma erased_tm_open_tm_wrt_tm: forall W a R x, erased_tm W a R -> erased_tm W (open_tm_wrt_tm a (a_Var_f x)) R.
+Lemma roleing_tm_open_tm_wrt_tm: forall W a R x, roleing W a R -> roleing W (open_tm_wrt_tm a (a_Var_f x)) R.
 Proof.
   intros W a R x H.
-  pose K := erased_lc H.
+  pose K := roleing_lc H.
   rewrite open_tm_wrt_tm_lc_tm; eauto.
 Qed.
 
-Hint Resolve erased_tm_open_tm_wrt_tm : erased.
+Hint Resolve roleing_tm_open_tm_wrt_tm : roleing.
 
 
 Lemma Par_Pi_exists: ∀ x W rho (A B A' B' : tm) R R',
@@ -461,7 +463,7 @@ Proof.
   dependent induction H; eauto.
   - dependent induction H0; eauto.
     erewrite close_tm_wrt_tm_open_tm_wrt_tm; eauto.
-    constructor. eapply erased_Pi_some_any; eauto.
+    constructor. eapply roleing_Pi_some_any; eauto.
     apply mp_step with (b := a_Pi rho a R (close_tm_wrt_tm x b)); auto.
     + eapply Par_Pi_exists; eauto.
     + apply IHmultipar; auto.
@@ -474,8 +476,8 @@ Proof.
     assert (uniq ([(x,R)] ++ W)). {eapply multipar_rctx_uniq; eauto. }
     rewrite (tm_subst_tm_tm_intro x B (a_Var_f x0)); auto.
     replace ([(x0,R)] ++ W) with (nil ++ [(x0,R)] ++ W); auto.
-    eapply subst_tm_erased. simpl_env. apply erased_app_rctx.
-    solve_uniq. eapply multipar_erased_tm_fst; eauto.
+    eapply subst_tm_roleing. simpl_env. apply roleing_app_rctx.
+    solve_uniq. eapply multipar_roleing_tm_fst; eauto.
     econstructor. solve_uniq. auto. auto. 
 Qed.
 
@@ -524,30 +526,30 @@ Proof.
         rewrite close_tm_wrt_co_open_tm_wrt_co; auto.
         constructor. econstructor; eauto 1.
         intros. rewrite (co_subst_co_tm_intro c).
-        apply subst_co_erased. auto. auto. auto.
+        apply subst_co_roleing. auto. auto. auto.
         apply mp_step with (b:= (a_CPi (Eq a0 a1 b R) a)); eauto.
         econstructor; eauto 2. intros. constructor.
         rewrite (co_subst_co_tm_intro c).
-        apply subst_co_erased. auto. auto. auto.
+        apply subst_co_roleing. auto. auto. auto.
       * eapply mp_step with (b:= (a_CPi (Eq a0 a1 T R) (close_tm_wrt_co c b))); eauto.
         -- apply Par_CPi_exists; auto 2. constructor.
-           eapply multipar_erased_tm_fst; eauto.
+           eapply multipar_roleing_tm_fst; eauto.
         -- apply IHmultipar; eauto.
            ++ rewrite fv_co_co_tm_close_tm_wrt_co_rec.
               fsetdec.
            ++ rewrite open_tm_wrt_co_close_tm_wrt_co; auto.
       + eapply mp_step with (b:= (a_CPi (Eq a0 b T R) a)); eauto.
         -- eapply (Par_CPi (singleton c)); eauto 2.
-           constructor. eapply multipar_erased_tm_fst; eauto.
+           constructor. eapply multipar_roleing_tm_fst; eauto.
            intros. constructor. rewrite (co_subst_co_tm_intro c).
-           apply subst_co_erased. auto. eapply multipar_erased_tm_fst; eauto.
+           apply subst_co_roleing. auto. eapply multipar_roleing_tm_fst; eauto.
            auto.
   - apply mp_step with (b:= (a_CPi (Eq b B T R) a)); auto.
      eapply (Par_CPi (singleton c)); eauto.
-     constructor. eapply multipar_erased_tm_fst; eauto.
-     constructor. eapply multipar_erased_tm_fst; eauto.
+     constructor. eapply multipar_roleing_tm_fst; eauto.
+     constructor. eapply multipar_roleing_tm_fst; eauto.
      intros. constructor. rewrite (co_subst_co_tm_intro c).
-     apply subst_co_erased. auto. eapply multipar_erased_tm_fst; eauto.
+     apply subst_co_roleing. auto. eapply multipar_roleing_tm_fst; eauto.
      auto. Unshelve. apply (fv_co_co_tm a). apply (fv_co_co_tm a).
 Qed.
 
@@ -577,7 +579,7 @@ Proof.
   intros W A B a A' B' a' T T' R R1 R' H.
   dependent induction H; eauto.
   - inversion H; subst. split. constructor; auto.
-    split. all:constructor; eauto. econstructor. eapply erased_sub; eauto.
+    split. all:constructor; eauto. econstructor. eapply roleing_sub; eauto.
   - inversion H; subst.
     eapply IHmultipar; eauto.
     destruct (IHmultipar _ _ _ _ _ _ _ _ _ _ ltac:(auto) ltac:(auto))
@@ -600,10 +602,10 @@ Proof.
   dependent induction H; eauto 2.
   - autorewrite with lngen. constructor.
     assert (uniq ([(x,R)] ++ W)). {eapply rctx_uniq; eauto. }
-    apply erased_a_Abs with (L := union (singleton x) (dom W)).
+    apply role_a_Abs with (L := union (singleton x) (dom W)).
     intros. rewrite (tm_subst_tm_tm_intro x B (a_Var_f x0)); auto.
     replace ([(x0,R)] ++ W) with (nil ++ [(x0,R)] ++ W); auto.
-    apply subst_tm_erased with (R1 := R). simpl_env. apply erased_app_rctx.
+    apply subst_tm_roleing with (R1 := R). simpl_env. apply roleing_app_rctx.
     solve_uniq. auto. econstructor; auto. solve_uniq.
   - assert (Par W (a_UAbs rho R B) (a_UAbs rho R (close_tm_wrt_tm x b)) R0).
     eapply (Par_Abs_exists); auto.
@@ -624,9 +626,9 @@ Proof.
   intros c W a a' R e H.
   dependent induction H; eauto 1.
   - rewrite close_tm_wrt_co_open_tm_wrt_co; auto.
-    econstructor. apply erased_a_CAbs with (L := fv_co_co_tm a).
+    econstructor. apply role_a_CAbs with (L := fv_co_co_tm a).
     intros. rewrite (co_subst_co_tm_intro c); auto.
-    apply subst_co_erased. auto. auto.
+    apply subst_co_roleing. auto. auto.
   - apply mp_step with (b := ((a_UCAbs (close_tm_wrt_co c b)))); eauto.
     apply Par_CAbs_exists; auto.
     apply IHmultipar; eauto.
@@ -666,12 +668,15 @@ Qed.
 
 Lemma Par_Path : forall F a R W a', Path F a R -> Par W a a' R -> Path F a' R.
 Proof. intros. generalize dependent a'. induction H; intros.
+       - inversion H0; subst. eauto. have E: (Ax a' A0 R1 = Cs A).
+         eapply binds_unique; eauto using uniq_toplevel.
+         inversion E.
        - inversion H1; subst. eauto. have E: (Ax a A R1 = Ax a' A0 R2).
          eapply binds_unique; eauto using uniq_toplevel.
          inversion E. subst. contradiction.
        - inversion H1; subst. eauto. apply IHPath in H9.
          inversion H9. apply IHPath in H9. econstructor; auto.
-         apply Par_erased_tm_snd in H10. eapply erased_lc; eauto.
+         apply Par_roleing_tm_snd in H10. eapply roleing_lc; eauto.
        - inversion H0; subst. eauto. apply IHPath in H3. inversion H3.
          apply IHPath in H3. econstructor; auto.
 Qed.
