src/FcEtt/ett_path.v
@@ -7,12 +7,15 @@ Require Export FcEtt.ett_inf.
 Require Export FcEtt.ett_ott.
 Require Export FcEtt.ett_ind.
 Require Import FcEtt.toplevel.
-Require Import FcEtt.ett_erased.
+Require Import FcEtt.ett_roleing.
 Require Import FcEtt.ext_wf.
 
-Lemma Path_binds_toplevel : forall F a R, Path F a R -> exists a0 A0 R0,
-                                   binds F (Ax a0 A0 R0) toplevel.
-Proof. intros. induction H. exists a, A, R1; auto. auto. auto.
+Lemma Path_binds_toplevel : forall F a R, Path F a R ->
+                     (exists A, binds F (Cs A) toplevel) \/
+                     (exists a0 A0 R0, binds F (Ax a0 A0 R0) toplevel
+                                                  /\ ~(SubRole R0 R)).
+Proof. intros. induction H. left. exists A; auto.
+       right. exists a, A, R1; auto. auto. auto.
 Qed.
 
 Lemma Path_subst : forall F a b R x, Path F a R -> lc_tm b ->
@@ -46,15 +49,12 @@ Proof. intros. induction a; simpl in H1; auto; try (inversion H1; fail).
           inversion H1; subst. eauto.
 Qed.
 
-Lemma Path_role_less : forall F a R, Path F a R -> exists a1 A1 R1,
-                          binds F (Ax a1 A1 R1) toplevel /\ ~(SubRole R1 R).
-Proof. intros F a R H. induction H; eauto.
-Qed.
-
 Lemma no_Path_reduction : forall R a F, Path F a R -> forall b, not (reduction_in_one a b R).
-Proof. 
+Proof.
   intros R a F H. induction H; simpl; intros.
   all : intros NH; inversion NH; subst.
+  - inversion H0; subst. assert (P : Ax b A0 R0 = Cs A).
+    eapply binds_unique; eauto using uniq_toplevel. inversion P.
   - inversion H1. subst. assert (P : Ax a A R1 = Ax b A0 R2).
     eapply binds_unique; eauto using uniq_toplevel. inversion P.
     subst. contradiction.
@@ -67,6 +67,7 @@ Qed.
 Lemma sub_Path : forall F a R1 R2, Path F a R1 -> SubRole R1 R2 ->
                         Path F a R2 \/ (exists a', reduction_in_one a a' R2).
 Proof. intros. induction H.
+        - left. eauto.
         - destruct (sub_dec R1 R2) as [P1 | P2].
           right. exists a. eauto. left. eauto.
         - apply IHPath in H0. inversion H0 as [P1 | P2].
@@ -80,21 +81,27 @@ Qed.
 Lemma nsub_Path : forall F a R1 R2, Path F a R1 -> SubRole R2 R1 ->
                         Path F a R2.
 Proof. intros. induction H.
+        - eauto.
         - destruct (sub_dec R1 R2) as [P1 | P2]. eauto. eauto.
         - apply IHPath in H0. eauto.
         - apply IHPath in H0. eauto.
 Qed.
 
-Lemma decide_Path : forall W a R, erased_tm W a R -> (exists F, Path F a R) \/
+Lemma decide_Path : forall W a R, roleing W a R -> (exists F, Path F a R) \/
                                      (forall F, not (Path F a R)).
 Proof.
   induction a; intros R' E.
   all: try solve [right; move => F h1; inversion h1].
   - inversion E; subst. apply IHa1 in H5. destruct H5 as [[F h0]|n].
-    left. exists F. econstructor; auto. eapply erased_lc; eauto.
+    left. exists F. econstructor; auto. eapply roleing_lc; eauto.
     right. intros. intro. inversion H; subst. pose (Q := n F). contradiction.
-  - inversion E; subst. destruct (sub_dec R R') as [P1 | P2].
-    right. intros. intro. inversion H; subst. have Q: (Ax a A R = Ax a0 A0 R1).
+  - inversion E; subst. left. exists F; eauto.
+    destruct (sub_dec R R') as [P1 | P2].
+    right. intros. intro. inversion H; subst.
+    have Q: (Ax a A R = Cs A0).
+    eapply binds_unique; eauto using uniq_toplevel.
+    inversion Q.
+    have Q: (Ax a A R = Ax a0 A0 R1).
     eapply binds_unique; eauto using uniq_toplevel.
     inversion Q. subst. contradiction. left. exists F. eauto.
   - inversion E; subst. apply IHa in H3. destruct H3 as [[F h0]|n].
@@ -102,19 +109,24 @@ Proof.
     pose (Q := n F). contradiction.
 Qed.
 
-Lemma Path_dec : forall W a R F, erased_tm W a R -> Path F a R \/ ~Path F a R.
+Lemma Path_dec : forall W a R F, roleing W a R -> Path F a R \/ ~Path F a R.
 Proof. induction a; intros R' E.
        all: try solve [right; move => h1; inversion h1].
         - intros. inversion H; subst. pose (P := IHa1 R' E H6).
           inversion P as [P1 | P2]. left; econstructor.
-          eapply erased_lc; eauto. auto. right. intro.
+          eapply roleing_lc; eauto. auto. right. intro.
           inversion H0; subst. contradiction.
-        - intros. inversion H; subst. pose (P := sub_dec R R').
-          inversion P as [P1 | P2]. right. intro.  inversion H0; subst.
+        - intros. inversion H; subst. destruct (E == F). subst.
+          left. eauto. right. intro. inversion H0; subst.
+          contradiction. contradiction.
+          pose (P := sub_dec R R').
+          inversion P as [P1 | P2]. right. intro. inversion H0; subst.
+          assert (Q : Ax a A R = Cs A0). eapply binds_unique; eauto.
+          eapply uniq_toplevel. inversion Q.
           assert (Ax a A R = Ax a0 A0 R1). eapply binds_unique; eauto.
           eapply uniq_toplevel. inversion H2; subst. contradiction.
           destruct (E == F). subst. left. eauto. right. intro.
-          inversion H0; subst. contradiction.
+          inversion H0; subst. contradiction. contradiction.
         - intros. inversion H; subst. pose (P := IHa R' E H4).
           inversion P as [P1 | P2]. left; eauto.
           right. intro. inversion H0; subst. contradiction.
