src/FcEtt/ett_roleing.v
@@ -1,0 +1,227 @@
+Set Bullet Behavior "Strict Subproofs".
+Set Implicit Arguments.
+
+Require Export FcEtt.tactics.
+Require Export FcEtt.imports.
+Require Import FcEtt.utils.
+
+Require Export FcEtt.ett_inf.
+Require Export FcEtt.ett_ott.
+Require Export FcEtt.ett_ind.
+
+
+Require Export FcEtt.ext_context_fv.
+
+Require Import FcEtt.ext_wf.
+Import ext_wf.
+Require Import FcEtt.param.
+
+Require Export FcEtt.toplevel.
+
+
+Lemma rctx_uniq : forall W a R, roleing W a R -> uniq W.
+Proof. intros W a R H. induction H; eauto.
+        - pick fresh x. eapply uniq_app_2; eauto.
+        - pick fresh c; eauto.
+Qed.
+
+Lemma roleing_app_rctx : forall W1 W2 W3 a R, uniq (W1 ++ W2 ++ W3) -> 
+                               roleing (W1 ++ W3) a R ->
+                               roleing (W1 ++ W2 ++ W3) a R.
+Proof. intros W1 W2 W3 a R U H. generalize dependent W2. 
+       dependent induction H; intros; eauto.
+        - eapply role_a_Abs with (L := union L (dom (W1 ++ W2 ++ W3))).
+          intros. rewrite <- app_assoc.
+          eapply H0; eauto. simpl_env. auto.
+        - eapply role_a_Pi with (L := union L (dom (W1 ++ W2 ++ W3))); eauto.
+          intros. rewrite <- app_assoc.
+          eapply H1; eauto. simpl_env. auto.
+        - econstructor; eauto.
+Qed.
+
+(* NOTE: we have a database 'roleing' for proving that terms are roleing. *)
+
+(* Tactics concerning roleing terms. *)
+
+Ltac roleing_pick_fresh x :=
+  match goal with
+    [ |- roleing ?W ?s ?R ] =>
+    let v := match s with
+             | a_UAbs _ _ _ => role_a_Abs
+             | a_Pi _ _ _ _ => role_a_Pi
+             | a_CPi _ _   => role_a_CPi
+             | a_UCAbs _   => role_a_CAbs
+             end
+    in pick fresh x and apply v
+  end.
+
+Ltac roleing_inversion :=
+  repeat match goal with
+  | [H : roleing _ (a_UAbs _ _ _) _ |- _ ] =>
+    inversion H; subst; clear H
+  | [H : roleing _ (a_App _ _ _ _) _ |- _ ] =>
+    inversion H; subst; clear H
+  | [H : roleing _ (a_Pi _ _ _ _) _ |- _ ] =>
+    inversion H; subst; clear H
+  | [H : roleing _ (a_CPi _ _) _ |- _ ] =>
+    inversion H; subst; clear H
+  | [H : roleing _ (a_UCAbs _ ) _ |- _ ] =>
+    inversion H; subst; clear H
+  | [H : roleing _ (a_CApp _ _) _ |- _ ] =>
+    inversion H; subst; clear H
+end.
+
+
+Inductive roleing_sort (W : role_context) : sort -> Prop := 
+| roleing_Tm : forall a R, roleing W a R -> roleing_sort W (Tm a R)
+| roleing_Co : forall a b A R, roleing W a R -> roleing W b R -> roleing W A R -> roleing_sort W (Co (Eq a b A R)).
+
+(* Check Forall_forall FIXME:?? *)
+
+
+Inductive roleing_context : role_context -> context -> Prop :=
+ | nil_roleing_ctx : roleing_context nil nil
+ | co_roleing_ctx : forall W G c a b A R,
+                   roleing_sort W (Co (Eq a b A R)) -> roleing_context W G -> 
+                   roleing_context W ([(c, (Co (Eq a b A R)))] ++ G)
+ | tm_roleing_ctx : forall W G x A R, roleing_context W G ->
+                   roleing_sort W (Tm A R) ->
+                   roleing_context ([(x,R)] ++ W) ([(x, (Tm A R))] ++ G).
+
+Lemma dom_rctx_le_ctx : forall G, dom (ctx_to_rctx G) [<=] dom G.
+Proof. intros. induction G. auto. destruct a, s; simpl; fsetdec.
+Qed.
+
+Lemma notin_ctx_rctx : forall x G, x `notin` (dom G) -> x `notin` dom (ctx_to_rctx G).
+Proof. intros. induction G. auto. destruct a, s; simpl in *.
+       all : pose (P := H); apply notin_add_2 in P; fsetdec.
+Qed.
+
+Lemma dom_roleing_ctx_rctx_le_ctx : forall W G, roleing_context W G ->
+                                               dom W [<=] dom G.
+Proof. intros; induction H; simpl; fsetdec.
+Qed.
+
+Lemma uniq_roleing_ctx_rctx : forall W G, roleing_context W G -> uniq G
+                                          -> uniq W.
+Proof. intros. induction H; auto.
+       apply IHroleing_context. eapply uniq_app_2; eauto.
+       inversion H0. apply IHroleing_context in H4. constructor.
+       auto. apply dom_roleing_ctx_rctx_le_ctx in H. fsetdec.
+Qed.
+
+Lemma roleing_lc : forall W a R, roleing W a R -> lc_tm a.
+intros; induction H; auto.
+Qed.
+
+Hint Resolve roleing_lc : lc.
+
+Lemma roleing_sub : forall W a R1 R2, roleing W a R1 -> SubRole R1 R2 ->
+                                     roleing W a R2.
+Proof. intros W a R1 R2 H S. generalize dependent R2. induction H; intros; eauto.
+       econstructor. auto. auto using param_covariant.
+Qed.
+
+Lemma subst_tm_roleing : forall W1 x R1 W2 a R b, 
+               roleing (W1 ++ [(x,R1)] ++ W2) a R ->
+               roleing W2 b R1 -> 
+               roleing (W1 ++ W2) (tm_subst_tm_tm b x a) R.
+Proof.
+  intros W1 x R1 W2 a R b H1 H2. dependent induction H1; simpl; eauto.
+  - destruct (x0 == x); auto. 
+     + subst. assert (P:R = R1).
+       eapply binds_mid_eq; eauto. subst. replace W1 with (nil ++ W1); eauto.
+       rewrite app_assoc. eapply roleing_app_rctx; simpl_env; eauto.
+       eapply roleing_sub; eauto.
+     + econstructor. eapply uniq_remove_mid; eauto.
+       eapply binds_remove_mid; eauto. eauto.
+  - pick fresh y and apply role_a_Abs.
+     rewrite tm_subst_tm_tm_open_tm_wrt_tm_var; auto 1.
+     rewrite <- app_assoc. eapply H0; eauto. simpl_env. auto.
+     eapply roleing_lc; eauto.
+  - pick fresh y and apply role_a_Pi; eauto.
+     rewrite tm_subst_tm_tm_open_tm_wrt_tm_var; auto 1.
+     rewrite <- app_assoc. eapply H0; eauto. simpl_env. auto.
+     eapply roleing_lc; eauto.
+  - pick fresh c and apply role_a_CPi; eauto.
+     rewrite tm_subst_tm_tm_open_tm_wrt_co_var; auto 1.
+     eapply H0; eauto. eapply roleing_lc; eauto.
+  - pick fresh c and apply role_a_CAbs; eauto.
+     rewrite tm_subst_tm_tm_open_tm_wrt_co_var; auto 1.
+     eapply H0; eauto. eapply roleing_lc; eauto.
+Qed.
+
+
+Lemma subst_co_roleing : forall W c g a R, lc_co g -> roleing W a R -> roleing W (co_subst_co_tm g c a) R.
+Proof.
+  intros W c g a R lc H. generalize dependent g.
+  induction H; intros; simpl; eauto.
+  - eapply role_a_Abs with (L := L).
+     intros x0 h1.
+     rewrite co_subst_co_tm_open_tm_wrt_tm_var; auto 2.
+   - eapply role_a_Pi with (L := L); eauto.
+     intros x0 h2.
+     rewrite co_subst_co_tm_open_tm_wrt_tm_var; auto 2.
+   - eapply role_a_CPi with (L := union L (singleton c)); eauto.
+     intros c0 h4.
+     rewrite co_subst_co_tm_open_tm_wrt_co_var; auto 2.
+   - eapply role_a_CAbs with (L := union L (singleton c)); eauto.
+     intros c0 h4.
+     rewrite co_subst_co_tm_open_tm_wrt_co_var; auto 2.
+Qed.
+
+Hint Resolve subst_tm_roleing subst_co_roleing : roleing.
+
+Lemma roleing_Pi_some_any: forall W x rho A R1 B R2,
+       x `notin` fv_tm_tm_tm B ->
+       roleing W A R2 ->
+       roleing ([(x,R1)] ++ W) (open_tm_wrt_tm B (a_Var_f x)) R2 ->
+       roleing W (a_Pi rho A R1 B) R2.
+Proof. intros. apply (role_a_Pi (union (singleton x) (dom W)));
+                 eauto using roleing_sub.
+       intros. rewrite (tm_subst_tm_tm_intro x B (a_Var_f x0)); auto.
+       replace ([(x0,R1)] ++ W) with (nil ++ [(x0,R1)] ++ W); auto.
+       assert (uniq ([(x,R1)] ++ W)). {eapply rctx_uniq; eauto. }
+       eapply subst_tm_roleing. simpl_env. apply roleing_app_rctx; eauto.
+       econstructor. solve_uniq. auto. auto.
+Qed.
+
+Lemma typing_roleing_mutual:
+    (forall G b A R, Typing G b A R -> roleing (ctx_to_rctx G) b R) /\
+    (forall G0 phi  (H : PropWff G0 phi ),
+        forall A B T R', phi = Eq A B T R' -> roleing (ctx_to_rctx G0) A R' /\ 
+        roleing (ctx_to_rctx G0) B R' /\ roleing (ctx_to_rctx G0) T Rep) /\
+     (forall G0 D p1 p2  (H : Iso G0 D p1 p2 ), True ) /\
+     (forall G0 D A B T R (H : DefEq G0 D A B T R), True) /\
+     (forall G0 (H : Ctx G0), True).
+Proof. 
+  apply typing_wff_iso_defeq_mutual; intros; repeat split; split_hyp; subst; 
+  simpl; auto.
+  all : try solve [inversion H2; subst; auto].
+  all : try solve [econstructor; eauto].
+  all : try solve [eauto using roleing_sub].
+  all : try solve [econstructor; eauto using ctx_to_rctx_uniq, ctx_to_rctx_binds_tm].
+  - destruct phi. move: (H0 a b A R0 eq_refl) => ?. split_hyp. clear H0.
+    eapply (@role_a_CPi L); eauto.
+  - inversion H2; subst. eapply roleing_sub. eauto. eauto.
+Qed.
+
+
+Lemma Typing_roleing: forall G b A R, Typing G b A R -> 
+                                     roleing (ctx_to_rctx G) b R.
+Proof.
+  apply typing_roleing_mutual.
+Qed.
+
+Hint Resolve Typing_roleing : roleing.
+
+Lemma toplevel_roleing1 : forall W F a A R, binds F (Ax a A R) toplevel -> 
+                                           uniq W -> roleing W a R.
+Proof.
+  intros.
+  move: (toplevel_closed H) => h0.
+  replace W with (nil ++ W ++ nil).
+  apply roleing_app_rctx. simpl_env; auto.
+  simpl_env. pose (P := Typing_roleing h0). simpl in P.
+  auto. simpl_env. auto.
+Qed.
