src/FcEtt/notations.v
@@ -17,8 +17,8 @@ Notation "Γ / D / ζ ⊨ a ⇒ b / R" := (Par Γ D ζ a b R) (at level 80, b at
 Notation "⊨ a ↝ b / R"  := (reduction_in_one a b R) (at level 80, b at level 35).
 
 (* Predicates *)
-(* Notation "ζ ⊨ 👻 a / R" := (erased_tm ζ a R) (at level 80, a at level 35). *)
-Notation "ζ ⊨ a : R" := (erased_tm ζ a R) (at level 80, a at level 35, R at level 35).
+(* Notation "ζ ⊨ 👻 a / R" := (roleing_tm ζ a R) (at level 80, a at level 35). *)
+Notation "ζ ⊨ a : R" := (roleing ζ a R) (at level 80, a at level 35, R at level 35).
 
 
 (* Other relations *)
